Make a bunch of functions and methods static

ironfleet/src/Dafny/Distributed/Common/Native/Io.s.dfy
@@ -138,15 +138,15 @@ class SharedStateIfc
 {
     // TODO: Replace this with a built-in type predicate.
     //       This would allow us to use datatypes and classes
-    predicate IsValueType<T>()
-    predicate {:axiom} ValueTypes()
+    static predicate IsValueType<T>()
+    static predicate {:axiom} ValueTypes()
         ensures IsValueType<bool>();
         ensures IsValueType<int>();
         ensures ValueTypes();
 
-    predicate IsValidLock(lock:Lock)           
+    static predicate IsValidLock(lock:Lock)           
 
-    method {:axiom} MakeLock(ghost env:HostEnvironment) returns (lock:Lock)
+    static method {:axiom} MakeLock(ghost env:HostEnvironment) returns (lock:Lock)
         requires env != null && env.Valid();
         modifies env.shared;
         modifies env.events;
@@ -155,7 +155,7 @@ class SharedStateIfc
         ensures  ToU(lock) !in old(env.shared.heap()) && ToU(lock) in env.shared.heap();
         ensures  forall ref :: ref in old(env.shared.heap()) ==> ref in env.shared.heap();
 
-    method {:axiom} Lock(lock:Lock, ghost env:HostEnvironment)
+    static method {:axiom} Lock(lock:Lock, ghost env:HostEnvironment)
         requires IsValidLock(lock);
         requires env != null && env.Valid();
         modifies env.shared;
@@ -164,7 +164,7 @@ class SharedStateIfc
         //ensures  env.shared.heap() == old(env.shared.heap())[ToU(lock) := ToU(true)];
         ensures  forall ref :: ref in old(env.shared.heap()) ==> ref in env.shared.heap();
 
-    method {:axiom} Unlock(lock:Lock, ghost env:HostEnvironment)
+    static method {:axiom} Unlock(lock:Lock, ghost env:HostEnvironment)
         requires IsValidLock(lock);
         requires env != null && env.Valid();
         modifies env.shared;
@@ -172,15 +172,15 @@ class SharedStateIfc
         ensures  env.events.history() == old(env.events.history()) + [SharedStateEvent(UnlockEvent(env.thread.ThreadId(), lock))];
         ensures  forall ref :: ref in old(env.shared.heap()) ==> ref in env.shared.heap();
 
-    predicate IsValidPtr<T>(ptr:Ptr<T>)
-    function  PtrInvariant<T>(ptr:Ptr<T>):iset<T>
+    static predicate IsValidPtr<T>(ptr:Ptr<T>)
+    static function  PtrInvariant<T>(ptr:Ptr<T>):iset<T>
     //function  GetPtr<T>(heap:SharedHeap, ptr:Ptr<T>) : T
 
-    predicate IsValidArray<T>(arr:Array<T>)
-    function  ArrayInvariant<T>(arr:Array<T>):iset<T>
-    function  Length<T>(arr:Array<T>):int
+    static predicate IsValidArray<T>(arr:Array<T>)
+    static function  ArrayInvariant<T>(arr:Array<T>):iset<T>
+    static function  Length<T>(arr:Array<T>):int
 
-    method {:axiom} MakePtr<T>(v:T, ghost ptr_invariant:iset<T>, ghost env:HostEnvironment) 
+    static method {:axiom} MakePtr<T>(v:T, ghost ptr_invariant:iset<T>, ghost env:HostEnvironment) 
         returns (ptr:Ptr<T>)
         requires ValueTypes() && IsValueType<T>();
         requires v in ptr_invariant;
@@ -193,7 +193,7 @@ class SharedStateIfc
         ensures  env.events.history() == old(env.events.history()) + [SharedStateEvent(MakePtrEvent(env.thread.ThreadId(), ToUPtr(ptr), ToU(v)))];
         ensures  forall ref :: ref in old(env.shared.heap()) ==> ref in env.shared.heap();
 
-    method {:axiom} ReadPtr<T>(ptr:Ptr<T>, ghost env:HostEnvironment) 
+    static method {:axiom} ReadPtr<T>(ptr:Ptr<T>, ghost env:HostEnvironment) 
         returns (v:T)
         requires IsValidPtr(ptr);
         requires env != null && env.Valid();
@@ -203,7 +203,7 @@ class SharedStateIfc
         ensures  env.events.history() == old(env.events.history()) + [SharedStateEvent(ReadPtrEvent(env.thread.ThreadId(), ToUPtr(ptr), ToU(v)))];
         ensures  forall ref :: ref in old(env.shared.heap()) ==> ref in env.shared.heap()
     
-    method {:axiom} WritePtr<T>(ptr:Ptr<T>, v:T, ghost env:HostEnvironment) 
+    static method {:axiom} WritePtr<T>(ptr:Ptr<T>, v:T, ghost env:HostEnvironment) 
         requires IsValidPtr(ptr);
         requires v in PtrInvariant(ptr);
         requires env != null && env.Valid();
@@ -212,7 +212,7 @@ class SharedStateIfc
         ensures  env.events.history() == old(env.events.history()) + [SharedStateEvent(WritePtrEvent(env.thread.ThreadId(), ToUPtr(ptr), ToU(v)))];
         ensures  forall ref :: ref in old(env.shared.heap()) ==> ref in env.shared.heap();
    
-    method {:axiom} ReadPtrAssume<T>(ptr:Ptr<T>, ghost env:HostEnvironment, ghost assumption:iset<SharedHeap>) 
+    static method {:axiom} ReadPtrAssume<T>(ptr:Ptr<T>, ghost env:HostEnvironment, ghost assumption:iset<SharedHeap>) 
         returns (v:T)
         requires IsValidPtr(ptr);
         requires env != null && env.Valid();
@@ -227,7 +227,7 @@ class SharedStateIfc
                                        + [SharedStateEvent(AssumeEvent (env.thread.ThreadId(), assumption))] ;
         ensures  forall ref :: ref in old(env.shared.heap()) ==> ref in env.shared.heap();
     
-    method {:axiom} MakeArray<T>(v:array<T>, ghost arr_invariant:iset<T>, ghost env:HostEnvironment) 
+    static method {:axiom} MakeArray<T>(v:array<T>, ghost arr_invariant:iset<T>, ghost env:HostEnvironment) 
         returns (arr:Array<T>)
         requires ValueTypes() && IsValueType<T>();
         requires v != null;
@@ -242,7 +242,7 @@ class SharedStateIfc
         ensures  env.events.history() == old(env.events.history()) + [SharedStateEvent(MakeArrayEvent(env.thread.ThreadId(), ToUArray(arr), ToU(v[..])))];
         ensures  forall ref :: ref in old(env.shared.heap()) ==> ref in env.shared.heap();
 
-    method {:axiom} ReadArray<T>(arr:Array<T>, index:int, ghost env:HostEnvironment) 
+    static method {:axiom} ReadArray<T>(arr:Array<T>, index:int, ghost env:HostEnvironment) 
         returns (v:T)
         requires IsValidArray(arr);
         requires 0 <= index < Length(arr);
@@ -253,7 +253,7 @@ class SharedStateIfc
         ensures  env.events.history() == old(env.events.history()) + [SharedStateEvent(ReadArrayEvent(env.thread.ThreadId(), ToUArray(arr), index, ToU(v)))];
         ensures  forall ref :: ref in old(env.shared.heap()) ==> ref in env.shared.heap()
     
-    method {:axiom} WriteArray<T>(arr:Array<T>, index:int, v:T, ghost env:HostEnvironment) 
+    static method {:axiom} WriteArray<T>(arr:Array<T>, index:int, v:T, ghost env:HostEnvironment) 
         requires IsValidArray(arr);
         requires 0 <= index < Length(arr);
         requires v in ArrayInvariant(arr);
@@ -263,7 +263,7 @@ class SharedStateIfc
         ensures  env.events.history() == old(env.events.history()) + [SharedStateEvent(WriteArrayEvent(env.thread.ThreadId(), ToUArray(arr), index, ToU(v)))];
         ensures  forall ref :: ref in old(env.shared.heap()) ==> ref in env.shared.heap();
     
-    method {:axiom} ReadArrayAssume<T>(arr:Array<T>, index:int, ghost env:HostEnvironment, ghost assumption:iset<SharedHeap>) 
+    static method {:axiom} ReadArrayAssume<T>(arr:Array<T>, index:int, ghost env:HostEnvironment, ghost assumption:iset<SharedHeap>) 
         returns (v:T)
         requires IsValidArray(arr);
         requires 0 <= index < Length(arr);
